backend/Debugvarproof.v
@@ -426,12 +426,12 @@ Qed.
 
 Inductive match_stackframes: Linear.stackframe -> Linear.stackframe -> Prop :=
   | match_stackframe_intro:
-      forall f sp rs c tf tc before after,
+      forall f cp sg sp rs c tf tc before after,
       match_function f tf ->
       match_code c tc ->
       match_stackframes
-        (Stackframe f sp rs c)
-        (Stackframe tf sp rs (add_delta_ranges before after tc)).
+        (Stackframe f cp sg sp rs c)
+        (Stackframe tf cp sg sp rs (add_delta_ranges before after tc)).
 
 Inductive match_states: Linear.state ->  Linear.state -> Prop :=
   | match_states_instr:
@@ -448,10 +448,10 @@ Inductive match_states: Linear.state ->  Linear.state -> Prop :=
       match_states (Callstate s f rs m)
                    (Callstate ts tf rs m)
   | match_states_return:
-      forall s rs m ts sg cp,
+      forall s rs m ts,
       list_forall2 match_stackframes s ts ->
-      match_states (Returnstate s rs m sg cp)
-                   (Returnstate ts rs m sg cp).
+      match_states (Returnstate s rs m)
+                   (Returnstate ts rs m).
 
 Lemma parent_locset_match:
   forall s ts,
@@ -532,34 +532,9 @@ Proof.
   }
   { erewrite <- find_comp_translated.
     inv TRF; unfold comp_of; simpl.
-    Set Nested Proofs Allowed.
-    Lemma call_trace_translated:
-      forall cp cp' vf ls tyargs t,
-        call_trace ge cp cp' vf ls tyargs t ->
-        call_trace tge cp cp' vf ls tyargs t.
-    Proof.
-      intros.
-      inv H.
-      - econstructor; eauto.
-      - econstructor; eauto.
-        apply Genv.find_invert_symbol.
-        rewrite symbols_preserved.
-        apply Genv.invert_find_symbol; eauto.
-        eauto. eapply eventval_list_match_preserved with (ge1 := ge) (ge2 := tge).
-        Set Printing Coercions.
-
-        intros; simpl.
-        unfold Genv.public_symbol. rewrite symbols_preserved.
-        unfold ge, tge. rewrite 2!Genv.globalenv_public. inv TRANSF; intuition.
-        rewrite H1. auto.
-        apply symbols_preserved.
-        auto.
-        Qed.
-
-    intros; subst.
-    eapply call_trace_translated; eauto.
-  }
-  constructor; auto. constructor; auto. constructor; auto.
+    eapply call_trace_eq; eauto using senv_preserved, symbols_preserved. }
+  constructor; auto. constructor; auto.
+  rewrite find_comp_translated; constructor; auto.
 - (* tailcall *)
   exploit find_function_translated; eauto. intros (tf' & A & B).
   exploit parent_locset_match; eauto. intros PLS.
@@ -627,11 +602,11 @@ Proof.
   erewrite <- match_stacks_call_comp; eauto.
   constructor; auto.
 - (* return *)
-  inv H5. inv H1.
+  inv H3. inv H1.
   econstructor; split.
   eapply plus_left. econstructor.
-  inv H6; auto.
-  inv H6. eapply return_trace_eq; eauto using senv_preserved.
+  inv H8; auto.
+  inv H8. eapply return_trace_eq; eauto using senv_preserved.
   apply eval_add_delta_ranges. traceEq.
   constructor; auto.
 Qed.
@@ -653,7 +628,7 @@ Lemma transf_final_states:
   forall st1 st2 r,
   match_states st1 st2 -> final_state st1 r -> final_state st2 r.
 Proof.
-  intros. inv H0. inv H. inv H7. econstructor; eauto.
+  intros. inv H0. inv H. inv H5. econstructor; eauto.
 Qed.
 
 Theorem transf_program_correct:
